# Higher order functions

## Foldl

Let's compare the type of left fold with the type of right fold.

``` haskell
foldr :: Foldable t => (a -> b -> b) -> b -> t a -> b
foldl :: Foldable t => (b -> a -> b) -> b -> t a -> b
```

The only visible difference is in the type of the combinator function.  The
function's first parameter is the already combined value and the second
parameter is the next value from the foldable.  Now let's see how it works.

Try out the following in ghci.
``` haskell
f :: (Show a, Integral a) => a -> String -> String
f n acc
  | even n = (show n) ++ acc
  | otherwise = acc

g :: (Show a, Integral a) => String -> a -> String
g acc n
  | even n = acc ++ (show n)
  | otherwise = acc

foldr f "" [1..6]
foldl g "" [1..6]
```

*g* is the same function as *f* with swapped parameters to conform to *foldl*
and accumulator is on the left side of concatenation operator.  To emphasize the
difference between the two folds, let's run the following.

``` haskell
foldr f "!" [1..6]
foldl g "!" [1..6]
```

So foldl would do something like this:

``` haskell
--foldr
(show 2 ++ (show 4 ++ (show 6 ++ "!")))

-- foldl
((("!" ++ show 2) ++ show 4) ++ show 6)
```

## Exercise
 * Write the *mysum :: (Num a, Foldable t) => t a -> a* function.

## Extra exercise
 * Implement *myfoldl*.

## Which fold should I use?

It is a hard question, and I can not give a complete answer to it because we
have not talked about lazy evaluation, which is a key factor.  For now follow
these guidelines:

 * If the foldable is an infinite structure you should use *foldr*.  We have not
   seen any infinite data structure so far.  You can start playing in ghci with
   *repeat, take, cycle* to have a basic understanding.
 * If the foldable is finite and it needs to be evaluated always completely,
   import *Data.List* and use *foldl'* which is identical to foldl.

